proofs/x86-64/avx2/ml_dsa_65/encoding/commitment.ec
@@ -1,0 +1,172 @@
+require import AllCore List IntDiv RealExp.
+
+from Jasmin require import JModel_x86.
+require import Bindings.
+
+from JazzEC require import Ml_dsa_65_avx2.
+from JazzEC require import Array256 Array128.
+from Spec require import GFq Rq Serialization Conversion Parameters VecMat MLDSA_W32_Rep.
+import BitEncoding BitChunking.
+
+import CDR Round Zq.
+
+require import ArrayExtra JWord_extra (* w2bitsE as int2bs *) EclibExtra (* size_flatten' *) JWordList (* nth_chunk *).
+ 
+(* Words of weird size should be cloned and bound here. *)
+lemma truncateu_32_4E (w : W32.t) : truncateu32_4 w = W4.bits2w (take 4 (W32.w2bits w)).
+proof.
+rewrite /truncateu32_4 W4.of_intE W32.to_uintE BS2Int.bs2int_mod //;congr.
+have {1}-> : 4 = size (take 4 (w2bits w)) by rewrite size_take //.
+by rewrite BS2Int.bs2intK.
+qed.
+
+op b_w1 = 15. (* 2^w1_bits - 1 *)
+lemma ilog_b_w1 : ilog 2 b_w1 = w1_bits - 1 by rewrite /b_w1 /=.
+
+(* Circuit spec  *)
+
+op commitment_encode_polynomial_lane(c : W32.t) : W4.t = 
+    truncateu32_4  c.
+
+
+lemma SimpleBitPack_liftE (p : wpoly) :
+  wpoly_urng b_w1 p =>
+    SimpleBitPack (liftu_wpoly p) b_w1
+  = to_list
+  (init_128_8
+     (fun (i0 : int) =>
+        W8.init
+          (fun (j : int) =>
+             (init_256_4 (fun (i1 : int) => commitment_encode_polynomial_lane p.[i1])).[(i0 * 8 + j) %/ 4].[
+             (i0 * 8 + j) %% 4]))).
+proof.
+move=> h @/SimpleBitPack; (pose l := ilog 2 _) => /=.
+have := ilog_b_w1; rewrite /bits_w1 /= => ?.
+have ? : size
+   (flatten (map (fun (x : W32.t) => IntegerToBits (asint (incoeff (to_uint x))) (l + 1)) (to_list p))) = 256*4.
++  rewrite  (size_flatten_ctt (l+1)).
+  +  by move => x; rewrite mapP => Hx;elim Hx => xw /= [? ->]; rewrite /IntegerToBits BS2Int.size_int2bs //.
+  by rewrite size_map /= size_to_list  /l /= /#.
+
+rewrite /BitsToBytes !array256_mapE /=.
+rewrite  -map_comp &(eq_sym) -map_comp /(\o) /=.
+apply (eq_from_nth witness); 1: by rewrite size_to_list /= size_map size_iota /#. 
+move => i; rewrite size_to_list => Hi.
+rewrite get_to_list (nth_map witness) /=; 1: by rewrite size_iota /#.
+rewrite wordP => j jb.
+rewrite !initiE //= initiE 1:/# /= get_bits2w // nth_take // 1:/# nth_drop;2: by smt().
++ rewrite nth_iota /#. 
+rewrite (nth_flatten false (l+1)).
++ by rewrite allP => x;rewrite mapP => Hx;elim Hx => xw /= [? ->]; rewrite /IntegerToBits BS2Int.size_int2bs //.
+rewrite nth_iota 1:/#  (nth_map witness) /=; 1: by rewrite size_to_list /= /#. 
+rewrite /commitment_encode_polynomial_lane .
+pose v:=p.[(i * 8 + j) %/ 4].
+have -> : p.[(8 * i + j) %/ (l + 1)] = v by smt().
+move: h => @/wpoly_urng /array256_allP /(_ v _) //= /=.
++ rewrite /to_list /mkseq mapP; exists ((i * 8 + j) %/ 4); smt(mem_iota).
+move => h. 
+rewrite incoeffK truncateu_32_4E get_bits2w 1:/#.
+rewrite nth_take 1,2:/#. 
+rewrite /IntegerToBits w2bitsE /l ilog_b_w1 /bitlenqm1md /= (modz_small _ q) 1:/# /BS2Int.int2bs.
+by rewrite !nth_mkseq 1,2:/# /= /#.
+qed. 
+
+lemma commitment_encode_polynomial _a :
+   hoare [ M.commitment____encode_polynomial :
+       commitment = _a /\ wpoly_urng b_w1 _a
+     ==>
+       to_list res = SimpleBitPack (liftu_wpoly _a) b_w1
+   ].
+proc => /=;inline *.
+proc change 1 : { temp <- W64.of_int 4097;}; 1: by auto.
+proc change 2 : { shift <- zeroextu256 temp; }.
++ auto => &1 &2 ->; rewrite /VMOV_64 zeroextu256E zeroextu256E.
+  rewrite wordP => i ib.
+  rewrite pack2E pack2E pack4E initiE 1:/# /= initiE 1:/# /= initiE 1:/# /= initiE 1:/# /=.
+  case (i %/ 64 = 0) => ?; 1: by rewrite ifT 1:/# initiE 1:/# /= get_of_list /#.
+  case (i %/ 128 = 0) => ?; 2: by auto.
+  rewrite initiE 1:/# /= get_of_list 1:/#.
+  by have -> /= : (i %% 128 %/ 64) = 1 by smt().
+
+proc change ^while.1 : { c0 <- sliceget256_32_256 commitment (input_offset*8);};1: by auto;smt().
+proc change ^while.3 : { c1 <- sliceget256_32_256 commitment (input_offset*8);};1: by auto;smt().
+proc change ^while.5 : { c2 <- sliceget256_32_256 commitment (input_offset*8);};1: by auto;smt().
+proc change ^while.7 : { c3 <- sliceget256_32_256 commitment (input_offset*8);};1: by auto;smt().
+proc change ^while.9 : { c4 <- sliceget256_32_256 commitment (input_offset*8);};1: by auto;smt().
+proc change ^while.11 : { c5 <- sliceget256_32_256 commitment (input_offset*8);};1: by auto;smt().
+proc change ^while.13 : { c6 <- sliceget256_32_256 commitment (input_offset*8);};1: by auto;smt().
+proc change ^while.15 : { c7 <- sliceget256_32_256 commitment (input_offset*8);};1: by auto;smt().
+
+proc change ^while.28 : {encoded <- sliceset128_8_256 encoded (output_offset*8) c0;}; 1: by auto;smt().
+
+unroll for ^while.
+cfold 5.
+wp -2.
+
+conseq (:  commitment = init_256_32 (fun i => zeroextu4_32 (truncateu32_4 _a.[i])) ==>
+    encoded  = let mapped = init_256_4 (fun i => commitment_encode_polynomial_lane _a.[i]) in
+    init_128_8 (fun i => W8.init (fun j => mapped.[(i*8+j) %/ 4].[(i*8+j) %% 4]))); last by circuit. 
+
++ move => &hr [->+]; rewrite /wpoly_urng allP => ?.
+  by rewrite tP => k kb; rewrite initiE 1:/# /= /zeroextu4_32 /truncateu32_4 /= of_uintK /= modz_small 1:/# to_uintK.
++ by move => &hr [<- Hrng] ? /= => ->;rewrite SimpleBitPack_liftE //=.
+  
+qed.
+
+import VecMat PolyKVec.
+
+require import Array768 Array1536.
+
+op  input_unflatten(a : 'a Array1536.t) =
+     KArray.init (fun i => Array256.of_list witness (sub a (256*i) 256)).
+op  output_unflatten(a : 'a Array768.t) =
+     KArray.init (fun i => Array128.of_list witness (sub a (128*i) 128)).
+
+lemma commitment_encode _a :
+    kvec = 6 =>
+    hoare [ M.commitment____encode :
+       commitment = _a /\ wpolykvec_urng (input_unflatten _a) b_w1 
+     ==>
+       output_unflatten res = 
+           KArray.map (fun (p : poly) => Array128.of_list witness (SimpleBitPack  p b_w1)) (liftu_wpolykvec (input_unflatten _a))
+   ].
+move => Hkvec.
+proc => /=.
+while (0 <= i <= 6 /\ commitment = _a /\ wpolykvec_urng (input_unflatten _a) b_w1  /\
+       forall k, 0 <= k < i =>
+       (output_unflatten encoded_commitment).[k] =
+       (map (fun (p : poly) => Array128.of_list witness (SimpleBitPack  p b_w1)) (liftu_wpolykvec (input_unflatten _a))).[k]);
+       last first.
+       + auto => /> &hr *;do split;1: smt().
+         move => r0 j0 *;rewrite tP => k kb; smt().
+wp; ecall (commitment_encode_polynomial (Array256.init (fun (i_0 : int) => _a.[i * 256 + i_0]))).
+auto => /> &hr ?? Hrng H ?;do split. 
++ move : Hrng; rewrite /wpolykvec_urng /wpoly_urng !allP /=  => Hrng ii iib.
+  have := Hrng i{hr} _; 1:smt().
+  rewrite allP /= /input_unflatten initiE 1:/# /= => Hrngj.
+  have := Hrngj ii _; 1:smt().
+  rewrite initiE 1:/# /= initiE 1:/# /= nth_sub 1:/# /#. 
+move => ? rr Hrr; do split;1,2: smt().
+move => k kbl kbh.
+case(0<=k<i{hr}) => *.
++ 
+   have -> : (output_unflatten
+   (Array768.init
+      (fun (ii : int) => if i{hr} * 128 <= ii < i{hr} * 128 + 128 then rr.[ii - i{hr} * 128] else encoded_commitment{hr}.[ii]))).[k] =
+    ((output_unflatten encoded_commitment{hr})).[k]; last by smt().
+  rewrite !initiE 1..2:/# /= /of_list /= tP => kk kkb.
+  rewrite !initiE 1,2:/# !nth_sub 1,2:/# initiE 1:/# /= /#.
+have -> : k = i{hr} by smt().
++ have -> : 
+   (output_unflatten
+   (Array768.init
+      (fun (ii : int) => if i{hr} * 128 <= ii < i{hr} * 128 + 128 then rr.[ii - i{hr} * 128] else encoded_commitment{hr}.[ii]))).[i{hr}]  =
+    (rr); last first.
+  + have <- := Array128.to_listK witness rr;rewrite Hrr mapiE 1:/# /=;congr;congr.
+    rewrite /liftu_wpolykvec mapiE 1:/#;congr;rewrite /input_unflatten initiE 1:/# /=.
+    rewrite tP => kk kkb; rewrite !initiE 1,2:/# /= nth_sub /#.
+ 
+rewrite initiE 1:/# /= tP => ii iib.
+rewrite  initiE 1:/# /= nth_sub 1:/# initiE 1:/# /= /#.
+qed.
+
