proofs/x86-64/avx2/ml_dsa_65/ml_dsa_65_avx2_barray.ec
@@ -6828,8 +6828,8 @@ module M = {
     var temp:W64.t;
     var shift:W256.t;
     var encoding_shuffles:W256.t;
-    var input_offset:W64.t;
-    var output_offset:W64.t;
+    var input_offset:int;
+    var output_offset:int;
     var c0:W256.t;
     var c1:W256.t;
     var c2:W256.t;
@@ -6842,25 +6842,25 @@ module M = {
     shift <- (zeroextu256 (VMOV_64 temp));
     shift <- (VPBROADCAST_16u16 (truncateu16 shift));
     encoding_shuffles <- commitment__ENCODING_SHUFFLES;
-    input_offset <- (W64.of_int 0);
-    output_offset <- (W64.of_int 0);
-    while ((input_offset \ult (W64.of_int ((256 * 32) %/ 8)))) {
-      c0 <- (BArray1024.get256d commitment (W64.to_uint input_offset));
-      input_offset <- (input_offset + (W64.of_int 32));
-      c1 <- (BArray1024.get256d commitment (W64.to_uint input_offset));
-      input_offset <- (input_offset + (W64.of_int 32));
-      c2 <- (BArray1024.get256d commitment (W64.to_uint input_offset));
-      input_offset <- (input_offset + (W64.of_int 32));
-      c3 <- (BArray1024.get256d commitment (W64.to_uint input_offset));
-      input_offset <- (input_offset + (W64.of_int 32));
-      c4 <- (BArray1024.get256d commitment (W64.to_uint input_offset));
-      input_offset <- (input_offset + (W64.of_int 32));
-      c5 <- (BArray1024.get256d commitment (W64.to_uint input_offset));
-      input_offset <- (input_offset + (W64.of_int 32));
-      c6 <- (BArray1024.get256d commitment (W64.to_uint input_offset));
-      input_offset <- (input_offset + (W64.of_int 32));
-      c7 <- (BArray1024.get256d commitment (W64.to_uint input_offset));
-      input_offset <- (input_offset + (W64.of_int 32));
+    input_offset <- 0;
+    output_offset <- 0;
+    while ((output_offset < ((4 * 256) %/ 8))) {
+      c0 <- (BArray1024.get256d commitment input_offset);
+      input_offset <- (input_offset + 32);
+      c1 <- (BArray1024.get256d commitment input_offset);
+      input_offset <- (input_offset + 32);
+      c2 <- (BArray1024.get256d commitment input_offset);
+      input_offset <- (input_offset + 32);
+      c3 <- (BArray1024.get256d commitment input_offset);
+      input_offset <- (input_offset + 32);
+      c4 <- (BArray1024.get256d commitment input_offset);
+      input_offset <- (input_offset + 32);
+      c5 <- (BArray1024.get256d commitment input_offset);
+      input_offset <- (input_offset + 32);
+      c6 <- (BArray1024.get256d commitment input_offset);
+      input_offset <- (input_offset + 32);
+      c7 <- (BArray1024.get256d commitment input_offset);
+      input_offset <- (input_offset + 32);
       c0 <- (VPACKUS_8u32 c0 c1);
       c1 <- (VPACKUS_8u32 c2 c3);
       c2 <- (VPACKUS_8u32 c4 c5);
@@ -6872,8 +6872,8 @@ module M = {
       c0 <- (VPACKUS_16u16 c0 c1);
       c0 <- (VPERMQ c0 (W8.of_int 216));
       c0 <- (VPSHUFB_256 c0 encoding_shuffles);
-      encoded <- (BArray128.set256d encoded (W64.to_uint output_offset) c0);
-      output_offset <- (output_offset + (W64.of_int 32));
+      encoded <- (BArray128.set256d encoded output_offset c0);
+      output_offset <- (output_offset + 32);
     }
     return encoded;
   }
